%! Author = tstreule

\section*{General}

\subsection*{Formeln}
%
\textbf{Circle}: $U\ped{circle} = 2\pi r$, $A\ped{circle} = \pi r^2$

%	\textbf{Laplace}:\\
%	\begin{tabular}{ c@{$\;\laplace\;$}c c c@{$\;\laplace\;$}c }
%		$f(at)$			& $\frac{1}{\abs{a}}F(s/a)$	&& $f(t-a)$		& $\eu^{-as}F(s)$\\
%		$f(t)\eu^{at}$	& $F(s-a)$					&& $f'(t)$		& $sF(s) - f(0^+)$\\
%		$t^n$			& $n!/s^{n+1}$				&& $t^n f(t)$	& $(-1)^n F^{(n)}(s)$\\
%		$\sin(at)$		& $\frac{a}{s^2 + a^2}$		&& $\cos(at)$	& $\frac{s}{s^2 + a^2}$\\
%		$\eu^{at}$		& $\frac{1}{s - a}$			&& $t^n \eu^{at}$& $\frac{n!}{(s-a)^{n+1}}$
%	\end{tabular}

\textbf{Constants}:\\
\begin{tabular}{r@{$\;=\;$}l}
    $h$			& $\unit[6.626 {\scriptstyle\mathrm{E}-34}]{Js} = \unit[4.135 {\scriptstyle\mathrm{E}-15}]{eV\,s}$,
    \quad $\hbar = \frac{h}{2\pi}$,
    \quad $hc = \unit[1.986 {\scriptstyle\mathrm{E}-25}]{Jm}$\\
    $\epsilon_0$& $\unitfrac[8.85 {\scriptstyle\mathrm{E}-5}]{As}{Vm}$\\
    $\mu_0$		& $\unitfrac[4\pi {\scriptstyle\mathrm{E}-7}]{N}{A^2}$\\
    $k\ped{B}$	& $\unitfrac[1.38 {\scriptstyle\mathrm{E}-23}]{J}{K} = \unitfrac[8.617 {\scriptstyle\mathrm{E}-5}]{eV}{K}$\\
    $q$			& $\unit[1.602 {\scriptstyle\mathrm{E}-19}]{C}$, \quad $m_e = \unit[9.109 {\scriptstyle\mathrm{E}-31}]{kg}$, \quad $m_p = \unit[1.672 {\scriptstyle\mathrm{E}-27}]{kg}$\\
    $F$			& $\unitfrac[96485]{C}{mol}$ (Faraday)\\ % charge of 1 mole of electrons
    $R$         & $N\ped{A} k\ped{B} = \unitfrac[8.314]{J}{mol\;K}$ (Ideal gas constant)\\
    $N\ped{A}$	& $\unitfrac[6.022 {\scriptstyle\mathrm{E}23}]{particles}{mol}$
    \qquad $\SI{0}{\degreeCelsius} = \unit[273.15]{K}$
\end{tabular}
%%%%%%%%%%%%%%%%%%%%%%%%%%%%%%%%%%%%%%%%%%%%%%%%%%%%%%
\subsection*{Einheiten}
%
\formula{Druck}{\unit[1]{Pa} = \unitfrac[1]{N}{m^2} = \unitfrac[1]{J}{m^3} = \unitfrac[10]{g}{cm\cdot s^2}}\\
\formula{Induktivität}{\unit[1]{H} = \unitfrac[1]{Vs}{A} = \unit[1]{\Omega\,s}}\\
\formula{Power}{\unit[1]{W} = \unitfrac[1]{J}{s} = \unit[1]{VA}}\\
\formula{electron volt}{\unit[1]{eV} = \unit[1.602 {\scriptstyle\mathrm{E}-19}]{J} = \unitfrac[23.06]{kcal}{mol}}\\
\formula{Charge}{\SI{1}{\coulomb} = \SI{1}{\ampere\second}}\\
\formula{Energy}{\SI{1}{\joule} = \unitfrac[1]{kg\;m^2}{s^2} = \unit[1]{Nm} = \unit[1]{VAs} = \unit[1]{CV} = \unit[1]{Ws}}\\
%%%%%%%%%%%%%%%%%%%%%%%%%%%%%%%%%%%%%%%%%%%%%%%%%%%%%%
\subsection*{Good to know}
%
\formula{Power in \unit{dB}}{10\,\log_{10}\frac{I}{I_0}}\\
\formula[\unit{\frac{\!W}{m^2}}]{Intensity}{ I = \frac{\textrm{avg. Power }(P)}{\textrm{area }(A)} }\\
\formula[\unit{W} = \unit{\frac{kg\,m^2}{s^3}}]{avg. Power}{P = \frac{\textrm{avg. Work in cycle }(\overline{W})}{\textrm{cycle }(T)}}\\
\formula[\unit{J}=\unit{Ws}]{(avg.) Work}{\overline{W} = \int_{\textrm{cycle}} \frac{1}{\textrm{cycle} (T)} \cdot \vec{F}\cdot\vec{x} \diff t }\\

mass $m$ vibrates with an amplitude $a$ along $x$-axis:\\
$\vec{x}(t) = a\sin(\omega t)\cdot \vec{e}_x, \quad \omega = 2\pi f = 2\pi/T, \quad \vec{F}(t) = m\,\ddot{\vec{x}}(t)$
%%%%%%%%%%%%%%%%%%%%%%%%%%%%%%%%%%%%%%%%%%%%%%%%%%%%%%
\subsection*{NuS}
%
\formula{Induktivität}{u(t) = L \deriv{i_L}{t} \enskip\laplace\enskip U(s) = sL\,I_L(s)}\\
\formula{Konduktivität}{i(t) = C \deriv{u_C}{t} \enskip\laplace\enskip U(s) = \frac{1}{sC}\,U_C(s)}\\

\formula{Transformator}{u_1 = L_1 \deriv{i_1}{t} - M \deriv{i_2}{t} \textnormal{,\enskip $M$: mutual inductance}}\\
\formula{LCR-Schwingkreis}{\omega_0 = 2\pi f_0 = 1/\sqrt{LC}}\\
%%%%%%%%%%%%%%%%%%%%%%%%%%%%%%%%%%%%%%%%%%%%%%%%%%%%%%
\subsection*{Laplace}
%	%Laplace Transformation: \;
%	$\phantom{\laplace} \dis{0.4} u(t)=\mathcal{L}^{-1}\{U(s)\} = \frac{1}{2\pi\iu} \int_{\bar{s}}^s U(s)\eu^{st} \diff s$\\
%	$\laplace \dis{0.4} U(s)=\mathcal{L}\{u(t)\} = \int_0^\infty u(t)\eu^{-st} \diff t$
%
\begin{tabular}{ rcl }
    \toprule
%		$u(t)$							& \laplace	& $U(s)$								\\%\addlinespace
%		\midrule
    $\lambda\;u(t) + \mu\;v(t)$		& \laplace	& $\lambda\;U(s) + \mu\;V(s)$			\\
    ${u(at),\; \scriptstyle a>0}$	& \laplace	& $\frac{1}{a}$ $U(\frac{s}{a})$		\\
    { \color{red} $u(t-t_0)$ }		& \laplace	& $\eu^{-st_0}$ $U(s)$					\\
    $\eu^{-at}$ $u(t)$				& \laplace	& { \color{red} $U(s+a)$ }				\\
    ${ (-t)^{n} u(t) }$				& \laplace	& $U^{(n)}(s)$							\\
    $u^{(n)}(t)$					& \laplace	& $ {s^nU(s) - \ldots - u^{(n-1)}(0)} $	\\
    \midrule
%		$t^n$							& \laplace	& $\frac{n!}{s^{n+1}}$					\\\addlinespace
%		$\eu^{-at}$						& \laplace	& $\frac{1}{s+a}$						\\\addlinespace
%		$t\eu^{-at}$					& \laplace	& $\frac{1}{(s+a)^2}$					\\\addlinespace
%		$t^n\eu^{-at}$					& \laplace	& $\frac{n!}{(s+a)^{n+1}}$				\\\addlinespace
%		$\sin (at)$						& \laplace	& $\frac{a}{s^2+a^2}$					\\\addlinespace
%		$\cos(at)$						& \laplace	& $\frac{s}{s^2+a^2}$					\\\addlinespace
    \multicolumn{3}{c}{
        \begin{minipage}{.45\columnwidth} \centering
        \begin{tabular}{ ccc }
%					$u(t)$							& \laplace	& $U(s)$								\\%\addlinespace
%					\midrule
            $t^n$							& \laplace	& $\frac{n!}{s^{n+1}}$					\\
            $\eu^{-at}$						& \laplace	& $\frac{1}{s+a}$						\\
            $t\eu^{-at}$					& \laplace	& $\frac{1}{(s+a)^2}$					\\
        \end{tabular}
        \end{minipage}%
        \begin{minipage}{.45\columnwidth} \centering
        \begin{tabular}{ ccc }
%					$u(t)$							& \laplace	& $U(s)$								\\%\addlinespace
%					\midrule
            $t^n\eu^{-at}$					& \laplace	& $\frac{n!}{(s+a)^{n+1}}$				\\
            $\sin (at)$						& \laplace	& $\frac{a}{s^2+a^2}$					\\
            $\cos(at)$						& \laplace	& $\frac{s}{s^2+a^2}$					\\
        \end{tabular}
        \end{minipage}
    }\\
    \bottomrule
\end{tabular}
